\Question{\currfilebase}

\begin{enumerate}
    \item Let \(y = 0\), and we have
          \[
              f(x + 0) = f(x) = f(x) f(0),
          \]
          so either \(f(x) = 0\) or \(f(0) = 1\) for all \(x\).

          Assume, B.W.O.C., that \(f(0) \neq 1\), then we must have \(f(x) = 0\) for all \(x\), which means \(f'(x) = 0\), contradicting with \(f'(0) = k \neq 0\).

          Hence, \(f(0) = 1\).

          By definition of the derivative, we have
          \begin{align*}
              f'(x) & = \lim_{h \to 0} \frac{f(x + h) - f(x)}{h}  \\
                    & = \lim_{h \to 0} \frac{f(x) f(h) - f(x)}{h} \\
                    & = f(x) \lim_{h \to 0} \frac{f(h) - 1}{h},
          \end{align*}
          and letting \(x = 0\), we also have
          \[
              k = f'(0) = f(0) \lim_{h \to 0} \frac{f(h) - 1}{h} = \lim_{h \to 0} \frac{f(h) - 1}{h},
          \]
          and hence
          \[
              f'(x) = k f(x)
          \]
          as desired.

          This differential equation solves to
          \[
              f(x) = A e^{kx},
          \]
          and with the condition \(f(0) = 1\), we have \(A = 1\), and hence
          \[
              f(x) = e^{kx}
          \]
          for all \(x\).

    \item Let \(y = 0\), and we have
          \[
              g(x + 0) = g(x) = \frac{g(x) + g(0)}{1 + g(x) g(0)}.
          \]

          This means that
          \[
              g(x) + g(x)^2 g(0) = g(x) + g(0),
          \]
          which gives
          \[
              g(0) \left[g(x)^2 - 1\right] = 0.
          \]

          Since \(\abs*{g(x)} < 1\) for all \(x\), we must have \(g(x)^2 - 1 < 0\), and hence \(g(0) = 0\).

          By the definition of the derivative,
          \begin{align*}
              g'(x) & = \lim_{h \to 0} \frac{g(x + h) - g(x)}{h}                                  \\
                    & = \lim_{h \to 0} \frac{\frac{g(x) + g(h)}{1 + g(x) g(h)} - g(x)}{h}         \\
                    & = \lim_{h \to 0} \frac{g(x) + g(h) - g(x) - g(x)^2 g(h)}{h (1 + g(x) g(h))} \\
                    & = \lim_{h \to 0} \frac{g(h) \left[1 - g(x)^2\right]}{h (1 + g(x) g(h))}     \\
                    & = \left[1 - g(x)^2\right] \lim_{h \to 0} \frac{g(h)}{h (1 + g(x) g(h))}.
          \end{align*}

          Considering the limit, we have
          \begin{align*}
              \lim_{h \to 0} \frac{g(h)}{h (1 + g(x) g(h))} & = \lim_{h \to 0} \frac{g(h) / h}{1 + g(x) g(h)}                                          \\
                                                            & = \frac{\lim_{h \to 0} \left[g(h) / h\right]}{\lim_{h \to 0} \left[1 + g(x) g(h)\right]} \\
                                                            & = \frac{\lim_{h \to 0} \left[g(h) / h\right]}{1}                                         \\
                                                            & = \lim_{h \to 0} \frac{g(h)}{h},
          \end{align*}
          and hence
          \[
              g'(x) = \left[1 - g(x)^2\right] \lim_{h \to 0} \frac{g(h)}{h}.
          \]

          Let \(x = 0\), and we have
          \[
              k = g'(0) = 1 \cdot \lim_{h \to 0} \frac{g(h)}{h},
          \]
          hence giving the differential equation
          \[
              g'(x) = k \left[1 - g(x)^2\right].
          \]

          This rearranges to give
          \[
              \frac{\Diff g(x)}{1 - g(x)^2} = k \Diff x,
          \]
          and hence
          \[
              \left[\frac{1}{1 + g(x)} + \frac{1}{1 - g(x)}\right] \Diff g(x) = 2 k \Diff x,
          \]
          which gives
          \[
              \ln \abs*{1 + g(x)} - \ln \abs*{1 - g(x)} = 2kx + C.
          \]

          Let \(x = 0\), we have \(g(0) = 0\), and hence \(C = 0\), and hence
          \[
              \frac{1 + g(x)}{1 - g(x)} = \exp(2kx),
          \]
          and hence
          \[
              1 + g(x) = \exp(2kx) - \exp(2kx) g(x),
          \]
          which gives
          \[
              g(x) = \frac{\exp(2kx) - 1}{\exp(2kx) + 1} = \frac{\exp(kx) - \exp(-kx)}{\exp(kx) + \exp(-kx)} = \tanh(kx).
          \]
\end{enumerate}