\Question{\currfilebase}
\begin{enumerate}
    \item Since \(u = \cosh x\), \(\cosh 2x = 2 \cosh^2 x - 1 = 2 u^2 - 1\), and \(\sinh x \Diff x = \Diff \cosh x = \Diff u\). Hence,
          \begin{align*}
              \int \frac{\sinh x}{\cosh 2x} \Diff x & = \int \frac{\Diff u}{2 u^2 - 1}                                                          \\
                                                    & = \int \frac{1}{2} \left(\frac{1}{\sqrt{2}u - 1} - \frac{1}{\sqrt{2}u + 1}\right) \Diff u \\
                                                    & = \frac{1}{2\sqrt{2}} \left(\ln\abs*{\sqrt{2}u - 1} - \ln\abs*{\sqrt{2}u + 1}\right) + C  \\
                                                    & = \frac{1}{2\sqrt{2}} \ln\abs*{\frac{\sqrt{2}\cosh x - 1}{\sqrt{2}\cosh x + 1}} + C,
          \end{align*}
          as desired.

    \item Let \(u = \sinh x\), \(\cosh 2x = 1 + 2\sinh^2 x = 1 + 2u^2\), and \(\cosh x \Diff x = \Diff \sinh x = \Diff u\). Hence,
          \begin{align*}
              \int \frac{\cosh x}{\cosh 2x} \Diff x & = \int \frac{\Diff u}{1 + 2u^2}                      \\
                                                    & = \frac{1}{\sqrt{2}}\arctan()\sqrt{2}u) + C          \\
                                                    & = \frac{1}{\sqrt{2}} \arctan()\sqrt{2} \sinh x) + C.
          \end{align*}

    \item Notice that
          \[
              \frac{\cosh x}{\cosh 2x} - \frac{\sinh x}{\cosh 2x} = \frac{2e^{-x}}{e^{2x} + e^{-2x}} = \frac{2e^{x}}{1 + e^{4x}}.
          \]

          Let \(u = e^x\), \(\Diff u = \Diff e^x = e^x \Diff x\), and therefore
          \begin{align*}
              \int_{0}^{1} \frac{\Diff u}{1 + u^4} & = \int_{-\infty}^{0} \frac{e^x \Diff x}{1 + x^4}                                                                                                                      \\
                                                   & = \frac{1}{2} \int_{-\infty}^{0} \frac{\cosh x}{\cosh 2x} - \frac{\sinh x}{\cosh 2x} \Diff x                                                                          \\
                                                   & = \frac{1}{2} \left[\frac{1}{\sqrt{2}} \arctan(\sqrt{2} \sinh x) - \frac{1}{2\sqrt{2}} \ln\abs*{\frac{\sqrt{2}\cosh x - 1}{\sqrt{2}\cosh x + 1}}\right]_{-\infty}^{0} \\
                                                   & = \frac{1}{4\sqrt{2}} \left[2\arctan(\sqrt{2} \sinh x) - \ln\abs*{\frac{\sqrt{2}\cosh x - 1}{\sqrt{2}\cosh x + 1}}\right]_{-\infty}^{0}                               \\
                                                   & = \frac{1}{4\sqrt{2}} \left[\left(0 - \ln \abs*{\frac{\sqrt{2} - 1}{\sqrt{2} + 1}}\right) - \left(2 \cdot (-\frac{\pi}{2}) - \ln\abs*{1}\right)\right]                \\
                                                   & = \frac{1}{4\sqrt{2}} \left[\pi - 2\ln(\sqrt{2} - 1)\right]                                                                                                           \\
                                                   & = \frac{\pi + 2\ln(\sqrt{2} + 1)}{4\sqrt{2}},
          \end{align*}
          as desired.
\end{enumerate}