\Question{\currfilebase}

\begin{enumerate}
    \item Since \(A, Q, C\) lie on a straight line, \(\vect{AQ} = \lambda \vect{AC}\) for some \(\lambda \in \RR\). This means
          \[
              q - a = \lambda (c - a),
          \]
          and hence
          \[
              \frac{q - a}{c - a} = \lambda \in \RR,
          \]
          as required.

          Hence, we must have
          \[
              \frac{q - a}{c - a} = \left(\frac{q - a}{c - a}\right)^* = \frac{q^* - a^*}{c^* - a^*}.
          \]

          Cross-multiplying the terms out give
          \[
              (c - a)(q^* - a^*) = (c^* - a^*)(q - a)
          \]
          exactly as desired.

          Substituting in \(a^* = 1 / a\) and \(c^* = 1 / c\), we have
          \[
              (c - a) \left(q^* - \frac{1}{a}\right) = \left(\frac{1}{c} - \frac{1}{a}\right)(q - a),
          \]
          and expanding the brackets gives
          \[
              cq^* - aq^* - \frac{c}{a} + 1 = \frac{q}{c} - \frac{a}{c} - \frac{q}{a} + 1,
          \]
          and hence
          \[
              cq^* - aq^* - \frac{c}{a} = \frac{q}{c} - \frac{a}{c} - \frac{q}{a}.
          \]

          Multiplying by \(ac\) on both sides gives us
          \[
              a c^2 q^* - a^2 c q^* - c^2 = aq - a^2 - cq,
          \]
          and hence
          \[
              ac (c - a) q^* = (a - c)q - (a^2 - c^2) = (a - c)q - (a - c)(a + c).
          \]

          We can divide through \((a - c)\) on both sides since \(a \neq c\). Hence,
          \[
              0 = q - (a + c) + ac q^*,
          \]
          and hence
          \[
              acq^* + q = a + c,
          \]
          as desired.

    \item By part 1, we must have
          \[
              acq^* + q = a + c, bdq^* + q = b + d.
          \]

          Since \(q = q\), we have
          \[
              acq^* - (a + c) = bdq^* - (b + d),
          \]
          and rearranging gives
          \[
              (ac - bd) q^* = (a + c) - (b + d),
          \]
          exactly as desired.

          We also have \(q^* = q^*\), and hence
          \[
              \frac{a + c - q}{ac} = \frac{b + d - q}{bd},
          \]
          which gives
          \[
              (bd)(a + c - q) = (ac)(b + d - q),
          \]
          and rearranging gives
          \[
              (ac - bd)q = ac(b + d) - bd(a + c).
          \]

          Summing this with previously, we have
          \[
              (ac - bd)(q + q^*) = (a + c) - (b + d) + ac(b + d) - bd(a + c).
          \]

          We notice that
          \begin{align*}
              (a + c) - (b + d) + ac(b + d) - bd(a + c) & = a + c - b - d + abc + acd - abd - bcd \\
                                                        & = a - b + acd - bcd + c - d + abc - abd \\
                                                        & = (a - b)(1 + cd) + (c - d)(1 + ab),
          \end{align*}
          and hence
          \[
              (ac - bd)(q + q^*) = (a - b)(1 + cd) + (c - d)(1 + ab),
          \]
          exactly as desired.

    \item By part 1, we must have
          \[
              p + abp^* = a + b.
          \]

          Since \(p\) is real, \(p = p^*\), and hence
          \[
              (1 + ab)p = a + b,
          \]
          as desired.

          Similarly, we must have
          \[
              (1 + cd)q = c + d,
          \]
          and putting this back into the result from part 2, we have
          \[
              (ac - bd)(q + q^*) = \frac{(a - b)(c + d)}{p} + \frac{(c - d)(a + b)}{p},
          \]
          and hence since \(ac - bd \neq 0\), we have
          \begin{align*}
              p(q + q^*) & = \frac{(a - b)(c + d) + (c - d)(a + b)}{ac - bd}       \\
                         & = \frac{ac + ad - bc - bd + ac + bc - ad - bd}{ac - bd} \\
                         & = \frac{2ac - 2bd}{ac - bd}                             \\
                         & = 2,
          \end{align*}
          as desired.
\end{enumerate}