\Question{\currfilebase}

\begin{enumerate}
    \item By differentiating both sides of the second differential equation, we can see
          \begin{align*}
              \NdiffFrac{2}{y}{x} + g'(x) y + g(x) \DiffFrac{y}{x} & = \DiffFrac{u}{x}                                    \\
                                                                   & = h(x) - f(x) u                                      \\
                                                                   & = h(x) - f(x) \left(\DiffFrac{y}{x} + g(x) y\right),
          \end{align*}
          and hence rearranging gives
          \[
              \NdiffFrac{2}{y}{x} + (f(x) + g(x)) \DiffFrac{y}{x} + (g'(x) + f(x) g(x))y = f(x),
          \]
          as desired.

    \item We must have \(g(x) + f(x) = 1 + \frac{4}{x}\), and \(g'(x) + f(x) g(x) = \frac{2}{x} + \frac{2}{x^2}\), with \(h(x) = 4x + 12\).

          Hence, from the first equation, we have \(f(x) = 1 + \frac{4}{x} - g(x)\), and putting this into the second equation gives us
          \[
              g'(x) + \left(1 + \frac{4}{x} - g(x)\right) g(x) = \frac{2}{x} + \frac{2}{x^2}.
          \]

          If \(g(x) = k x^n\), then \(g'(x) = kn x^{n - 1}\), and putting this back we have
          \[
              knx^{n - 1} + \left(1 + \frac{4}{x} - kx^n\right) kx^n = \frac{2}{x} + \frac{2}{x^2},
          \]
          which gives
          \[
              -k^2 x^{2n} + kx^n + k(n + 4)x^{n - 1} = 2x^{-1} + 2x^{-2}.
          \]

          Therefore, we could simply let \(n = -1\), and \(k = 2\). Verify that
          \[
              \LHS = -4 x^{-2} + 2x^{-1} + 2 \cdot 3 x^{-2} = 2 x^{-1} + 2 x^{-2} = \RHS.
          \]

          Hence, \(g(x) = \frac{2}{x}\), and \(f(x) = 1 + \frac{2}{x}\).

          The differential equation for \(u\) is
          \[
              \DiffFrac{u}{x} + \left(1 + \frac{2}{x}\right)u = 4x + 12.
          \]

          The integration factor is
          \[
              I(x) = e^{\int (1 + \frac{2}{x}) \Diff x} = e^{x + 2 \ln x} = x^2 e^x,
          \]
          and hence
          \[
              x^2 e^x \DiffFrac{u}{x} + e^x (x^2 + 2x)u = \DiffFrac{x^2 e^x u}{x} = 4x^3 e^x + 12 x^2 e^x.
          \]

          Notice the right-hand side is the derivative of \(4x^3 e^x\), and hence
          \[
              x^2 e^x u = 4 x^3 e^x + C.
          \]

          When \(x = 1\),
          \begin{align*}
              \LEvalAt{u}{x = 1} & = \LEvalAt{\DiffFrac{y}{x}}{x = 1} + g(1) \LEvalAt{y}{x = 1} \\
                                 & = -3 + 2 \cdot 5                                             \\
                                 & = 7,
          \end{align*}
          and hence
          \[
              7e = 4e + C,
          \]
          giving \(C = 3e\).

          Hence,
          \[
              u = 4 x + \frac{3e}{x^2 e^x}.
          \]

          The differential equation for \(y\) gives
          \[
              \DiffFrac{y}{x} + \frac{2}{x} y = u,
          \]
          and hence the integration factor is \(x^2\), giving
          \[
              \DiffFrac{x^2 y}{x} = 4x^3 + 3e \cdot e^{-x},
          \]
          and hence by integration on both sides, we have
          \[
              x^2 y = x^4 - 3e \cdot e^{-x} + C'.
          \]

          Since when \(x = 1\), \(y = 5\), we must have
          \[
              5 = 1 - 3 + C',
          \]
          giving \(C' = 7\).

          Hence,
          \[
              x^2 y = x^4 - 3e^{1 - x} + 7,
          \]
          and hence
          \[
              y = x^2 - 3 x^{-2} e^{1 - x} + 7 x^{-2}.
          \]
\end{enumerate}