\Question{\currfilebase}

\begin{enumerate}
    \item By rearrangement, we have
          \[
              \frac{\Diff u}{u} = \left(1 + \frac{1}{x + 1}\right) \Diff x,
          \]
          and hence by integration,
          \[
              \ln \abs*{u} = x + \ln\abs*{x + 1} + C.
          \]

          This gives
          \[
              u = C (x + 1) e^x
          \]
          as the general solution.

    \item Since \(y = z e^{-x}\), we must have
          \[
              \DiffFrac{y}{x} = \DiffFrac{z}{x} e^{-x} - z e^{-x} = \left(\DiffFrac{z}{x} - z\right) e^{-x},
          \]
          and
          \[
              \NdiffFrac{2}{y}{x} = \NdiffFrac{2}{z}{x} e^{-x} - 2 \DiffFrac{z}{x} e^{-x} + z e^{-x} = \left(\NdiffFrac{2}{z}{x} - 2 \DiffFrac{z}{x} + z\right) e^{-x}.
          \]

          Hence, the original differential equation can be simplified:
          \begin{align*}
              (x + 1) \NdiffFrac{2}{y}{x} + x \DiffFrac{y}{x} - y                                                                            & = 0  \\
              (x + 1) \left(\NdiffFrac{2}{z}{x} - 2 \DiffFrac{z}{x} + z\right) e^{-x} + x \left(\DiffFrac{z}{x} - z\right) e^{-x} - z e^{-x} & = 0  \\
              (x + 1) \left(\NdiffFrac{2}{z}{x} - 2 \DiffFrac{z}{x} + z\right) + x \left(\DiffFrac{z}{x} - z\right) - z                      & = 0  \\
              (x + 1) \NdiffFrac{2}{z}{x} - (x + 2)\DiffFrac{z}{x}                                                                           & = 0,
          \end{align*}
          which is a first-order differential equation for \(\DiffFrac{z}{x}\).

          Hence, from part (i), we have the general solution to this differential equation is
          \[
              \DiffFrac{z}{x} = C(x + 1)e^x,
          \]
          and hence by integration
          \[
              z = C \int (x + 1) e^x \Diff x = C \left[\int x \Diff e^x + \int e^x \Diff x\right] = C [xe^x - e^x + e^x] + D.
          \]

          Therefore, \(y = z e^{-x} = De^{-x} + Cx\). Let \(A = C\) and \(B = D\) and this is exactly what is desired.

    \item The complementary function is the differential equation solved in the previous part. For the complementary function, consider \(y = ax^2 + b\), and hence \(\DiffFrac{y}{x} = 2ax\) and \(\NdiffFrac{2}{y}{x} = 2a\). Hence,
          \[
              2a(x + 1) + x \cdot 2ax - ax^2 - c = ax^2 + 2ax + (2a - c) = x^2 + 2x + 1.
          \]

          Hence, \(a = 1\) and \(c = 1\) giving \(y = x^2 + 1\) is a particular integral.

          Therefore, the general solution to the differential equation is
          \[
              y = Ax + Be^{-x} + x^2 + 1.
          \]
\end{enumerate}