\Question{\currfilebase}

\begin{enumerate}
    \item \begin{enumerate}
              \item By rearranging, we have
                    \[
                        x_{n + 1} = 1 + \frac{1}{x_n + 1},
                    \]
                    and \(x_n \geq 1\) for \(n = 0\).

                    If \(x_n \geq 1\) for some \(n = k \geq 0\), we must have \(\frac{1}{x_{k} + 1} > 0\), and hence
                    \[
                        x_{k + 1} = 1 + \frac{1}{x_k + 1} > 1,
                    \]
                    and so \(x_{k + 1} \geq 1\).

                    Hence, by the principle of mathematical induction, \(x_n \geq 1\) for all \(n \in \NN\).

              \item We have
                    \begin{align*}
                        x_{n + 1}^2 - 2 & = \left(1 + \frac{1}{x_n + 1}\right)^2 - 2                                           \\
                                        & = 1 + \frac{2}{x_n + 1} + \frac{1}{\left(x_n + 1\right)^2} - 2                       \\
                                        & = \frac{1 + 2 \left(x_n + 1\right) - \left(x_n + 1\right)^2}{\left(x_n + 1\right)^2} \\
                                        & = \frac{1 + 2 x_n + 2 - x_n^2 - 2x_n - 1}{\left(x_n + 1\right)^2}                    \\
                                        & = \frac{- x_n^2 + 2}{\left(x_n + 1\right)^2}                                         \\
                                        & = - \frac{x_n^2 - 2}{\left(x_n + 1\right)^2}.
                    \end{align*}

                    Since
                    \[
                        \frac{1}{\left(x_n + 1\right)^2} > 0,
                    \]
                    it must be \(x_{n + 1}^2 - 2\) and \(x_n^2 - 2\) must take opposite signs.

                    \begin{align*}
                        \abs*{x_{n + 1}^2 - 2} & = \frac{1}{\left(x_n + 1\right)^2} \abs*{x_n^2 - 2} \\
                                               & \leq \frac{1}{(1 + 1)^2} \abs*{x_n^2 - 2}           \\
                                               & = \frac{1}{4} \abs*{x_n^2 - 2}.
                    \end{align*}

              \item \(x_0^2 - 2 = -1 < 0\), and so \(x_n^2 - 2 < 0\) for all even \(n\), and \(> 0\) for all odd \(n\).

                    Hence, \(x_{10}^2 - 2 < 0\),and hence \(x_{10}^2 \leq 2\).

                    We have
                    \begin{align*}
                        \abs*{x_0^2 - 2} & = \abs*{1 - 2} = 1,                              \\
                        \abs*{x_1^2 - 2} & \leq \frac{1}{4} \abs*{x_0^2 - 2} = \frac{1}{4}, \\
                                         & \phantom{\leq}\vdots                             \\
                        \abs*{x_n^2 - 2} & \leq \frac{1}{4^n},
                    \end{align*}
                    and hence
                    \[
                        \abs*{x_10^2 - 2} \leq \frac{1}{4^{10}} = \frac{1}{2^{20}}.
                    \]

                    We have
                    \begin{align*}
                        2^{20} & = \left(2^{20}\right)^2 \\
                               & = 1024^2                \\
                               & > \left(10^3\right)^2   \\
                               & = 10^6,
                    \end{align*}
                    and so
                    \[
                        \abs*{x_{10}^2 - 2} = 2 - x_{10}^2 < 10^{-6},
                    \]
                    and hence
                    \[
                        2 - 10^{-6} < x_{10}^2 < 2,
                    \]
                    which gives
                    \[
                        2 - 10^{-6} \leq x_{10}^2 \leq 2.
                    \]
          \end{enumerate}

    \item \begin{enumerate}
              \item We have
                    \begin{align*}
                        y_{n + 1} - \sqrt{2} & = \frac{y_n^2 - 2\sqrt{2} y_n}{2 y_n}                            \\
                                             & = \frac{y_n^2 - 2 \sqrt{2} y_n + \left(\sqrt{2}\right)^2}{2 y_n} \\
                                             & = \frac{\left(y_n - \sqrt{2}\right)^2}{2 y_n}.
                    \end{align*}

                    \(y_n \geq 1\) is true for the base case \(n = 0\).

                    If it is true for \(n = k\),  we have
                    \[
                        \frac{\left(y_n - \sqrt{2}\right)^2}{2 y_n} \geq 0,                    \]
                    and so \(y_{n + 1} - \sqrt{2} \geq 0\), and hence \(y_{n + 1} \geq \sqrt{2} \geq 1\) as desired.

                    In fact, we can conclude that \(y_n \geq \sqrt{2}\) for all \(n \geq 1\).

              \item Since \(y_n \geq 1\), we have \(0 \leq \frac{1}{y_n} \leq 1\), and hence we have
                    \[
                        y_{n + 1} - \sqrt{2} \leq \frac{\left(y_n - \sqrt{2}\right)^2}{2}.
                    \]

                    We aim to show the desired result by induction on \(n\). The base case when \(n = 1\) is
                    \[
                        y_1 = \frac{y_0^2 + 2}{2 y_0} = \frac{1^2 + 2}{2} = \frac{3}{2},
                    \]
                    and
                    \[
                        \RHS = 2 \cdot \left(\frac{\sqrt{2} - 1}{2}\right)^{2 \cdot 1} = 2 \cdot \frac{2 + 1 - 2 \sqrt{2}}{4} = \frac{3}{2} - \sqrt{2},
                    \]
                    and hence
                    \[
                        \LHS = y_1 - \sqrt{2} = \frac{3}{2} - \sqrt{2} \leq \RHS
                    \]
                    as desired.

                    Now we assume the desired result is true for some \(n = k\). For \(n = k + 1\),
                    \begin{align*}
                        y_{k + 1} - \sqrt{2} & \leq \frac{\left(y_k - \sqrt{2}\right)^2}{2}                                    \\
                                             & \leq \frac{\left[2 \cdot \left(\frac{\sqrt{2} - 1}{2}\right)^{2^k}\right]^2}{2} \\
                                             & = \frac{4 \cdot \left(\frac{\sqrt{2} - 1}{2}\right)^{2^k \cdot 2}}{2}           \\
                                             & = 2 \cdot \left(\frac{\sqrt{2} - 1}{2}\right)^{2^{k + 1}},
                    \end{align*}
                    which is precisely the desired statement for \(n = k + 1\).

                    So the desired is true for the base case where \(n = 1\). Given it is true for some \(n = k\), it is true for \(n = k + 1\). Hence, by the principle of mathematical induction,
                    \[
                        y_n - \sqrt{2} \leq 2 \cdot \left(\frac{\sqrt{2} - 1}{2}\right)^{2^n}
                    \]
                    for all \(n \geq 1\).

              \item First, we have \(y_{10} \geq \sqrt{2}\) by the stronger bound found for the first part.

                    Additionally,
                    \begin{align*}
                        y_{10} - \sqrt{2} & \leq 2 \cdot \left(\frac{\sqrt{2} - 1}{2}\right)^{2^{10}} \\
                                          & \leq 2 \cdot \left(\frac{\frac{1}{2}}{2}\right)^{2^{10}}  \\
                                          & = 2 \cdot \left(\frac{1}{2^2}\right)^{2^{10}}             \\
                                          & = 2 \cdot \left(\frac{1}{2}\right)^{2^{10} \cdot 2}       \\
                                          & = \frac{2}{2^{2^{11}}}                                    \\
                                          & = \frac{1}{2^{2^{11} - 1}}.
                    \end{align*}

                    For the bound, notice that
                    \begin{align*}
                        \frac{1}{2^{2^{11} - 1}} & = \frac{1}{2^{2048 - 1}}              \\
                                                 & = \frac{1}{2^{2047}}                  \\
                                                 & < \frac{1}{2^{2040}}                  \\
                                                 & = \frac{1}{\left(2^{10}\right)^{204}} \\
                                                 & < \frac{1}{\left(10^{3}\right)^{204}} \\
                                                 & < \frac{1}{\left(10^{3}\right)^{200}} \\
                                                 & = \frac{1}{10^{600}},
                    \end{align*}
                    and so
                    \[
                        y_{10} \leq \sqrt{2} + 10^{-600}.
                    \]

                    Hence, we can conclude
                    \[
                        \sqrt{2} \leq y_{10} \leq \sqrt{2} + 10^{-600}
                    \]
                    as desired.
          \end{enumerate}
\end{enumerate}