\Question{\currfilebase}

\begin{enumerate}
    \item We have
    \begin{align*}
        \text{RHS} &= \frac{r+1}{r} \left(\frac{1}{\binom{n+r-1}{r}} - \frac{1}{\binom{n+r}{r}}\right)\\
        &= \frac{r+1}{r} \left(\frac{r! (n-1)!}{(n+r-1)!} - \frac{r! n!}{(n+r)!}\right)\\
        &= \frac{r+1}{r} \left(\frac{r! (n-1)! (n+r)}{(n+r)!} - \frac{r! (n-1)! n}{(n+r)!}\right)\\
        &= \frac{r+1}{r} \cdot \frac{r! (n-1)! (n+r) - r! (n-1)! n}{(n+r)!}\\
        &= \frac{r+1}{r} \cdot \frac{r! (n-1)! r}{(n+r)!}\\
        &= \frac{(r+1)! (n-1)! }{(n+r)!}\\
        &= \binom{n+r}{r+1}\\
        &= \text{LHS}
    \end{align*}
    as desired.

    Therefore,
    \begin{align*}
        \sum_{n = 1}^{+\infty} \frac{1}{\binom{n+r}{r+1}} &= \sum_{n = 1}^{+\infty} \frac{r+1}{r} \left(\frac{1}{\binom{n+r-1}{r}} - \frac{1}{\binom{n+r}{r}}\right)\\
        &= \frac{r+1}{r} \sum_{n = 1}^{+\infty} \left(\frac{1}{\binom{n+r-1}{r}} - \frac{1}{\binom{n+r}{r}}\right)\\
        &= \frac{r+1}{r} \left[\sum_{n = 0}^{+\infty} \frac{1}{\binom{n + r}{r}} - \sum_{n = 1}^{+\infty} \frac{1}{\binom{n + r}{r}}\right]\\
        &= \frac{r+1}{r} \frac{1}{\binom{0+r}{r}}\\
        &= \frac{r+1}{r},
    \end{align*}
    assuming the sum converges.

    When \(r = 2\), we have
    \[
        \sum_{n = 1}^{+\infty} \frac{1}{\binom{n+2}{3}} = \frac{3}{2}.
    \]

    When \(n = 1\), \(\frac{1}{\binom{1 + 2}{3}} = \frac{1}{1} = 1\).

    Therefore,
    \[
        \sum_{n = 2}^{+\infty} \frac{1}{\binom{n+2}{3}} = \frac{1}{2}
    \]
    as desired.

    \item Notice that
    \begin{align*}
        \frac{3!}{n^3} < \frac{1}{\binom{n+1}{3}} &\iff \frac{3!}{n^3} < \frac{3!}{(n+1)n(n-1)}\\
        &\iff n^3 > (n+1)n(n-1)\\
        &\iff n^3 > n(n^2 - 1)\\
        &\iff n^3 > n^3 - n\\
        &\iff n > 0,
    \end{align*}
    which is true.

    Also, notice that
    \begin{align*}
        \frac{20}{\binom{n+1}{3}} - \frac{1}{\binom{n+2}{5}} < \frac{5!}{n^3} &\iff \frac{5!}{(n+1)(n)(n-1)} - \frac{5!}{(n+2)(n+1)(n)(n-1)(n-2)} < \frac{5!}{n^3}\\
        &\iff \frac{(n+2)(n-2) - 1}{(n+2)(n+1)(n)(n-1)(n-2)} < \frac{1}{n^3}\\
        &\iff (n^2 - 5)n^3 < (n^2 - 4)(n^2 - 1)n\\
        &\iff n^5 - 5n^3 < n^5 - 5n^3 + 4n\\
        &\iff 4n > 0,
    \end{align*}
    which is true.

    Therefore, we have that
    \begin{align*}
        \sum_{n = 3}^{+\infty} \frac{3!}{n^3} &< \sum_{n = 3}^{+\infty} \frac{1}{\binom{n+1}{3}}\\
        &= \sum_{n = 2}^{+\infty} \frac{1}{\binom{n+2}{3}}\\
        &= \frac{1}{2},
    \end{align*}
    and therefore \(\sum_{n = 3}^{+\infty} \frac{1}{n^3} < \frac{1}{12}\), and \(\sum_{n = 1}^{+\infty} \frac{1}{n^3} < 1 + \frac{1}{8} + \frac{1}{12} = \frac{29}{24} = \frac{116}{96}.\)

    On the other hand, we have
    \begin{align*}
        \sum_{n = 3}^{+\infty} \frac{5!}{n^3} &< \sum_{n = 3}^{+\infty} \left[\frac{20}{\binom{n+1}{3}} - \frac{1}{\binom{n+2}{5}}\right]\\
        &= 20 \sum_{n = 2}^{+\infty} \frac{1}{\binom{n+2}{3}} - \sum_{n = 1}^{+\infty} \frac{1}{\binom{n+4}{5}}\\
        &= 20 \cdot \frac{1}{2} - \frac{5}{4}\\
        &= 10 - \frac{5}{4}\\
        &= \frac{35}{4},
    \end{align*}
    and therefore \(\sum_{n = 3}^{+\infty} \frac{1}{n^3} > \frac{7}{96}\), and \(\sum_{n = 1}^{+\infty} \frac{1}{n^3} > 1 + \frac{1}{8} + \frac{7}{96} = \frac{115}{96}\).

    Hence,
    \[
        \frac{115}{96} < \sum_{n = 1}^{+\infty} \frac{1}{n^3} < \frac{116}{96}
    \]
    as desired.
\end{enumerate}