\Question{\currfilebase}

\begin{enumerate}
    \item We have
    \begin{align*}
        T(x) &= \int_0^x \frac{\Diff u}{1 + u^2}\\
        &\xlongequal[\substack{u=0^+, v=+\infty\\
        u=x, v=\frac{1}{x}}]{\substack{u = \frac{1}{v}\\
        \Diff u = - \frac{1}{v^2} \Diff v}} \int_{+\infty}^{\frac{1}{x}} -\frac{1}{v^2} \cdot \frac{1}{1 + \frac{1}{v^2}} \Diff v\\
        &= \int_{\frac{1}{x}}^{+\infty} \frac{\Diff v}{1 + v^2}\\
        &= \int_{0}^{+\infty} \frac{\Diff v}{1 + v^2} - \int_{0}^{\frac{1}{x}} \frac{\Diff v}{1 + v^2}\\
        &= T_{\infty} - T(x^{-1}),
    \end{align*}
    as desired.

    \item When \(u \neq a^{-1}\), we have
    \begin{align*}
        \frac{\Diff v}{\Diff u} &= \frac{\Diff}{\Diff u} \frac{u+a}{1-au}\\
        &= \frac{1 \cdot (1-au) + a \cdot (u+a)}{(1-au)^2}\\
        &= \frac{1 - au + au + a^2}{(1-au)^2}\\
        &= \frac{1 + a^2}{(1-au)^2}.
    \end{align*}

    Also, notice that
    \begin{align*}
        \frac{1 + v^2}{1 + u^2} &= \frac{1 + \left(\frac{u + a}{1 - au}\right)^2}{1 + u^2}\\
        &= \frac{(1-au)^2 + (u+a)^2}{(1+u^2) (1-au)^2}\\
        &= \frac{1 - 2au + a^2u^2 + u^2 + 2au + a^2}{(1+u^2) (1-au)^2}\\
        &= \frac{(1 + a^2) (1 + u^2)}{(1 - au)^2 (1 + u^2)}\\
        &= \frac{1 + a^2}{(1 - au)^2}.
    \end{align*}

    Therefore, \(\frac{\Diff v}{\Diff u} = \frac{1 + v^2}{1 + u^2}\) as desired.

    Consider the substitution \(v = \frac{u + a}{1 - au}\). When \(u = 0\), \(v = a\). When \(u = x, v = \frac{x + a}{1 - ax}\). Therefore,
    \begin{align*}
        T(x) &= \int_0^x \frac{\Diff u}{1 + u^2}\\
        &= \int_a^{\frac{x+a}{1-ax}} \frac{1+u^2}{1+v^2} \cdot \frac{\Diff v}{1 + u^2}\\
        &= \int_a^{\frac{x+a}{1-ax}} \frac{\Diff v}{1 + v^2}\\
        &= \int_0^{\frac{x+a}{1-ax}} \frac{\Diff v}{1 + v^2} - \int_0^a \frac{\Diff v}{1 + v^2}\\
        &= T\left(\frac{x+a}{1-ax}\right) - T(a),
    \end{align*}
    as desired.

    If we substitute \(T(x) = T_{\infty} - T(x^{-1})\) and \(T(a) = T_{\infty} - T(a^{-1})\), we can see that
    \begin{align*}
        T(x) &= T\left(\frac{x+a}{1-ax}\right) - T(a)\\
        T_{\infty} - T(x^{-1}) &= T\left(\frac{x+a}{1-ax}\right) - \left[T_{\infty} - T(a^{-1})\right]\\
        T(x^{-1}) &= 2T_{\infty} - T\left(\frac{x+a}{1-ax}\right) - T(a^{-1}),
    \end{align*}
    as desired.

    Now, let \(y = x^{-1}\) and \(b = a^{-1}\). Then
    \begin{align*}
        \frac{x + a}{1 - ax} &= \frac{y^{-1} + b^{-1}}{1 - b^{-1} y^{-1}}\\
        &= \frac{b + y}{by - 1}.
    \end{align*}

    This gives us
    \[
        T(y) = 2T_{\infty} - T\left(\frac{b + y}{by - 1}\right) - T(b),
    \]
    as desired.

    \item Let \(y = b = \sqrt{3}\). We can easily verify that \(b > 0\) and \(y > \frac{1}{b}\). Therefore,
    \[
        T(\sqrt{3}) = 2 T_{\infty} - T\left(\frac{\sqrt 3 + \sqrt 3}{3 - 1}\right) - T(\sqrt{3}),
    \]
    which simplified, gives us \(T(\sqrt{3}) = \frac{2}{3} T_{\infty}\) as desired.

    In \(T(x) = T\left(\frac{x + a}{1 - ax}\right) - T(a)\), let \(x = a = \sqrt{2} - 1\), we can verify that \(a > 0\) and \(x < \frac{1}{a}\), therefore we have
    \begin{align*}
        T(\sqrt{2} - 1) &= T\left(\frac{(\sqrt{2} - 1) + (\sqrt{2} - 1)}{1 - (\sqrt{2} - 1) \cdot (\sqrt{2} - 1)}\right) - T(\sqrt{2} - 1),\\
        T(\sqrt{2} - 1) &= T\left(\frac{2\sqrt{2} - 2}{1 - \left(2 + 1 - 2\sqrt{2}\right)}\right) - T(\sqrt{2} - 1),\\
        T(\sqrt{2} - 1) &= T\left(\frac{2\sqrt{2} - 2}{2\sqrt{2} - 2}\right) - T(\sqrt{2} - 1),\\
        2T(\sqrt{2} - 1) &= T(1).
    \end{align*}

    In \(T(x) = T_{\infty} - T(x^{-1})\), let \(x = 1\). We have
    \begin{align*}
        T(1) &= T_{\infty} - T(1),\\
        2T(1) &= T_{\infty}.
    \end{align*}

    Therefore, \(T(\sqrt{2} - 1) = \frac{1}{4} T_{\infty}\), as desired.
\end{enumerate}