\Question{\currfilebase}

\begin{enumerate}
    \item First, note that
          \begin{align*}
              1 & = \sum_{x, y = 1}^{x = n} \Prob(X = x, Y = y)                    \\
                & = \sum_{x = 1}^{n} \sum_{y = 1}^{n} k(x + y)                     \\
                & = \sum_{x = 1}^{n} \sum_{y = 1}^{n} (kx + ky)                    \\
                & = \sum_{x = 1}^{n} \left(n \cdot kx + k\sum_{y = 1}^{n} y\right) \\
                & = nk\sum_{x = 1}^{n} x + nk\sum_{y = 1}^{n} y                    \\
                & = n^2 (n+1) k
          \end{align*}

          Therefore, \(k = \frac{1}{n^2(n+1)}\)

          \begin{align*}
              \Prob(X = x) & = \sum_{y = 1}^{n} \Prob(X = x, Y = y) \\
                           & = \sum_{y = 1}^{n} k(x + y)            \\
                           & = nkx + k\sum_{y = 1}^{n} y            \\
                           & = nkx + \frac{kn(n+1)}{2}              \\
                           & = \frac{x}{n(n+1)} + \frac{1}{2n}      \\
                           & = \frac{2x + n+1}{2n(n+1)},
          \end{align*}
          as desired.

          By symmetry, \(\Prob(Y = y) = \frac{2y + n+1}{2n(n+1)}\).

          We have
          \[
              \Prob(X = x) \cdot \Prob(Y = y) = \frac{(2x+n+1)(2y+n+1)}{4n^2(n+1)^2}.
          \]

          But \(\Prob(X = x, Y = y) = \frac{x+y}{n^2(n+1)}\) is not equal to this. So \(X\) and \(Y\) are not independent.

    \item By definition,
          \[
              \Cov(X, Y) = \Expt(XY) - \Expt(X)\Expt(Y).
          \]

          We have
          \begin{align*}
              \Expt(X) = \Expt(Y) & = \sum_{t = 1}^{n} t \cdot \Prob(X = t)                                   \\
                                  & = \sum_{t = 1}^{n} \frac{t \cdot (2t + n + 1)}{2n(n+1)}                   \\
                                  & = \frac{1}{n(n+1)} \sum_{t = 1}^{n} t^2 + \frac{1}{2n} \sum_{t = 1}^{n} t \\
                                  & = \frac{n(n+1)(2n+1)}{6n(n+1)} + \frac{n(n+1)}{4n}                        \\
                                  & = \frac{2n+1}{6} + \frac{n+1}{4}                                          \\
                                  & = \frac{4n+2+3n+3}{12}                                                    \\
                                  & = \frac{7n+5}{12},
          \end{align*}
          and
          \begin{align*}
              \Expt(XY) & = \sum_{x, y = 1}^{n} xy \cdot \Prob(X = x, Y = y)                                                                  \\
                        & = \sum_{x = 1}^{n} \sum_{y = 1}^{n} \frac{xy(x + y)}{n^2(n+1)}                                                      \\
                        & = \frac{1}{n^2(n+1)} \sum_{x = 1}^{n} \sum_{y = 1}^{n} xy(x + y)                                                    \\
                        & = \frac{1}{n^2(n+1)} \sum_{x = 1}^{n} \sum_{y = 1}^{n} (x^2y + xy^2)                                                \\
                        & = \frac{1}{n^2(n+1)} \left[\sum_{x = 1}^{n} x^2 \sum_{y = 1}^{n} y + \sum_{x = 1}^{n} x \sum_{y = 1}^{n} y^2\right] \\
                        & = \frac{1}{n^2(n+1)} \cdot 2 \cdot \frac{n(n+1)(2n+1)}{6} \cdot \frac{n(n+1)}{2}                                    \\
                        & = \frac{(2n+1)(n+1)}{6}.
          \end{align*}

          Therefore,
          \begin{align*}
              \Cov(X, Y) & = \Expt(XY) - \Expt(X)\Expt(Y)                                \\
                         & = \frac{(2n+1)(n+1)}{6} - \frac{(7n+5)^2}{144}                \\
                         & = \frac{48n^2 + 72n + 24}{144} - \frac{49n^2 + 70n + 25}{144} \\
                         & = \frac{-n^2 + 2n - 1}{144}                                   \\
                         & = -\frac{(n-1)^2}{144}                                        \\
                         & < 0,
          \end{align*}
          as desired.
\end{enumerate}