\Question{\currfilebase}

We have
\begin{align*}
    \sum_{m = 1}^{n} a_m (b_{m + 1} - b_m) &= \sum_{m = 1}^{n} a_m b_{m + 1} - \sum_{m = 1}^{n} a_m b_m\\
    &= -\sum_{m = 0}^{n - 1} b_{m + 1} a_{m + 1} + \sum_{m = 1}^{n} b_{m + 1} a_m\\
    &= -\sum_{m = 1}^{n} b_{m + 1} a_{m + 1} + \sum_{m = 1}^{n} b_{m + 1} a_m + a_{n + 1} b_{n + 1} - a_1 b_1\\
    &= a_{n + 1} b_{n + 1} - a_1 b_1 - \sum_{m = 1}^{n} b_{m + 1}(a_{m + 1} - a_m),
\end{align*}
as desired.

\begin{enumerate}
    \item Let \(a_m = 1\). On one hand, we have
    \begin{align*}
        \sum_{m = 1}^{n} a_m (b_{m + 1} - b_m) &= \sum_{m = 1}^{n} \left[\sin(m + 1) x - \sin mx\right]\\
        &= \sum_{m = 1}^{n} 2 \cos \left(\frac{(m + 1)x + mx}{2}\right) \sin \left(\frac{(m + 1)x - mx}{2}\right)\\
        &= 2 \sum_{m = 1}^{n} \cos \left(m + \frac{1}{2}\right)x \sin \frac{x}{2}\\
        &= 2 \sin \frac{x}{2} \sum_{m = 1}^{n} \cos \left(m + \frac{1}{2}\right)x.
    \end{align*}

    On the other hand, we have
    \begin{align*}
        \sum_{m = 1}^{n} a_m (b_{m + 1} - b_m) &= a_{n + 1} b_{n + 1} - a_1 b_1 - \sum_{m = 1}^{n} b_{m + 1} (a_{m + 1} - a_m)\\
        &= \sin (n + 1) x - \sin x.
    \end{align*}

    Therefore, by rearranging, we have
    \[
        \sum_{m = 1}^{n} \cos \left(m + \frac{1}{2}\right)x = \frac{1}{2} \left[\sin(n + 1)x - \sin x\right] \Cosec \frac{1}{2} x
    \]
    as desired.

    \item Let \(a_m = m\), and let \(b_m = \cos \left(m - \frac{1}{2}\right)x\). We have the identity
    \[
        \cos A - \cos B = - 2 \sin\left(\frac{A + B}{2}\right) \sin \left(\frac{A - B}{2}\right).
    \]
    Therefore, we have
    \begin{align*}
        \sum_{m = 1}^{n} a_m (b_{m + 1} - b_m) &= \sum_{m = 1}^{n} m \cdot \left[\cos \left(m + \frac{1}{2}\right)x - \cos \left(m - \frac{1}{2}\right)x\right]\\
        &= \sum_{m = 1}^{n} -2m \sin mx \sin \frac{1}{2}x\\
        &= -2 \sin \frac{1}{2} x \sum_{m = 1}^{n} m \sin mx, 
    \end{align*}
    and
    \begin{align*}
        &\phantom{=} \sum_{m = 1}^{n} a_m (b_{m + 1} - b_m)\\
        &= a_{n + 1} b_{n + 1} - a_1 b_1 - \sum_{m = 1}^{n} b_{m + 1} (a_{m + 1} - a_m)\\
        &= (n + 1) \cos \left(n + \frac{1}{2}\right)x - 1 \cdot \cos \frac{1}{2} x - \sum_{m = 1}^{n} \cos\left(m + \frac{1}{2}\right)x \cdot 1\\
        &= (n + 1) \cos \left(n + \frac{1}{2}\right)x - \cos \frac{1}{2} x - \sum_{m = 1}^{n} \cos\left(m + \frac{1}{2}\right)x\\
        &= (n + 1) \cos \left(n + \frac{1}{2}\right)x - \cos \frac{1}{2} x - \frac{1}{2}\left(\sin (n + 1)x - \sin x\right)\Cosec \frac{1}{2}x\\
        &= \frac{1}{2} \Cosec \frac{1}{2}x \left[2(n + 1) \cos \left(n + \frac{1}{2}\right)x \sin \frac{1}{2}x - 2 \cos \frac{1}{2}x \sin \frac{1}{2}x - \left(\sin (n + 1)x - \sin x\right)\right]\\
        &= \frac{1}{2} \Cosec \frac{1}{2}x \left[(n + 1) \left(\sin(n + 1)x - \sin nx\right) - (\sin x - \sin 0) - \left(\sin (n + 1)x - \sin x\right)\right]\\
        &= \frac{1}{2} \Cosec \frac{1}{2}x \left[n \sin(n + 1)x - (n + 1) \sin nx\right].
    \end{align*}

    Therefore, we have
    \begin{align*}
        -2 \sin \frac{1}{2} x \sum_{m = 1}^{n} m \sin mx &= \frac{1}{2} \Cosec \frac{1}{2}x \left[n \sin(n + 1)x - (n + 1) \sin nx\right]\\
        \sum_{m = 1}^{n} m \sin mx &= - \frac{1}{4} \Cosec^2 \frac{1}{2}x \left[n \sin(n + 1)x - (n + 1) \sin nx\right],
    \end{align*}
    and therefore, \(p = -\frac{1}{4}n\), \(q = \frac{1}{4}(n + 1)\).
\end{enumerate}