\Question{\currfilebase}

We notice
\[
    (z - \exp(i\theta)) (z - \exp(-i\theta)) = z^2 - (\exp(i\theta) + \exp(-i\theta))z + 1 = z^2 - 2z \cos \theta + 1.
\]

The \(2n\)-th roots of \(-1\) are \(z_r\), where \(r = 0, 1, \ldots, 2n - 1\),
\[
    z_r = \exp\left(i\left(\frac{\pi}{2n} + \frac{2r\pi}{2n}\right)\right) = \exp\left(i\pi \cdot \frac{1 + 2r}{2n}\right),
\]
and hence
\begin{align*}
    z^{2n} + 1 & = \prod_{r = 0}^{2n - 1} (z - z_r)                                                                                                                                                                                     \\
               & = \left[\prod_{r = 0}^{n - 1} \left(z - \exp\left(i\pi \cdot \frac{1 + 2r}{2n}\right)\right)\right] \cdot \left[\prod_{r = n}^{2n - 1} \left(z - \exp\left(i\pi \cdot \frac{1 + 2r}{2n}\right)\right)\right]           \\
               & = \left[\prod_{r = 0}^{n - 1} \left(z - \exp\left(i\pi \cdot \frac{1 + 2r}{2n}\right)\right)\right] \cdot \left[\prod_{r = 0}^{n - 1} \left(z - \exp\left(i\pi \cdot \frac{1 + 2(2n - 1 - r)}{2n}\right)\right)\right] \\
               & = \left[\prod_{r = 0}^{n - 1} \left(z - \exp\left(i\pi \cdot \frac{1 + 2r}{2n}\right)\right)\right] \cdot \left[\prod_{r = 0}^{n - 1} \left(z - \exp\left(i\pi \cdot \frac{-1-2r}{2n}\right)\right)\right]             \\
               & = \prod_{r = 0}^{n - 1} \left(z - \exp\left(i\pi \cdot \frac{1 + 2r}{2n}\right)\right) \left(z - \exp\left(i\pi \cdot \frac{-1-2r}{2n}\right)\right)                                                                   \\
               & = \prod_{r = 0}^{n - 1} \left(z^2 - 2z \cos \left(\frac{2r + 1}{2n} \pi\right) + 1\right)                                                                                                                              \\
               & = \prod_{r = 1}^{n} \left(z^2 - 2z \cos \left(\frac{2r - 1}{2n} \pi\right) + 1\right).
\end{align*}

\begin{enumerate}
    \item Let \(z = i\), since \(n\) is even, \(z^{2n} = i^{2n} = (i^2)^n = (-1)^n = 1\).
          \begin{align*}
              2 & = z^{2n} + 1                                                                          \\
                & = \prod_{r = 1}^{n} \left(i^2 - 2i \cos \left(\frac{2r - 1}{2n} \pi\right) + 1\right) \\
                & = \prod_{r = 1}^{n} 2i \cos \left(\frac{2r - 1}{2n} \pi\right)                        \\
                & = (2i)^n \prod_{r = 1}^{n} \cos \left(\frac{2r - 1}{2n} \pi\right)                    \\
                & = 2^n (-1)^{\frac{n}{2}} \prod_{r = 1}^{n} \cos \left(\frac{2r - 1}{2n} \pi\right),
          \end{align*}
          and therefore
          \[
              \prod_{r = 1}^{n} \cos \left(\frac{2r - 1}{2n} \pi\right) = 2^{1 - n} (-1)^{-\frac{n}{2}} = 2^{1 - n} (-1)^{\frac{n}{2}}.
          \]
    \item Notice that in the product where \(n\) is odd, let \(k = \frac{n + 1}{2}\), then the term of this product will be
          \begin{align*}
              z^2 - 2z \cos \left(\frac{(2k - 1) \pi}{2n}\right) + 1 & = z^2 - 2z \cos \left(\frac{(n + 1 - 1)\pi}{2n}\right) + 1 \\
                                                                     & = z^2 - 2z \cos \frac{\pi}{2} + 1                          \\
                                                                     & = z^2 + 1.
          \end{align*}

          Therefore, we have
          \begin{align*}
              (z^2 + 1) \sum_{r = 0}^{n - 1} (-1)^r z^{2r} & = z^2 + 1                                                                                                                \\
                                                           & = \prod_{r = 1}^{n} \left(z^2 - 2z \cos \left(\frac{2r - 1}{2n} \pi\right) + 1\right)                                    \\
                                                           & = \prod_{r = 1}^{\frac{n - 1}{2}} \left(z^2 - 2z \cos \left(\frac{2r - 1}{2n} \pi\right) + 1\right) (z^2 + 1)            \\
                                                           & \phantom{=} \prod_{r = \frac{n + 3}{2}}^{n} \left(z^2 - 2z \cos \left(\frac{2r - 1}{2n} \pi\right) + 1\right)            \\
                                                           & = \prod_{r = 1}^{\frac{n - 1}{2}} \left(z^2 - 2z \cos \left(\frac{2r - 1}{2n} \pi\right) + 1\right) (z^2 + 1)            \\
                                                           & \phantom{=} \prod_{r = 1}^{\frac{n - 1}{2}} \left(z^2 - 2z \cos \left(\frac{2(n + 1 - r) - 1}{2n} \pi\right) + 1\right),
          \end{align*}
          and hence
          \begin{align*}
              \sum_{r = 0}^{n - 1} (-1)^r z^{2r} & = \prod_{r = 1}^{\frac{n - 1}{2}} \left(z^2 - 2z \cos \left(\frac{2r - 1}{2n} \pi\right) + 1\right) \left(z^2 - 2z \cos \left(\frac{2(n + 1 - r) - 1}{2n} \pi\right) + 1\right) \\
                                                 & = \prod_{r = 1}^{\frac{n - 1}{2}} \left(z^2 - 2z \cos \left(\frac{2r - 1}{2n} \pi\right) + 1\right) \left(z^2 - 2z \cos \left(\frac{2n - 2r + 1}{2n} \pi\right) + 1\right)      \\
                                                 & = \prod_{r = 1}^{\frac{n - 1}{2}} \left(z^2 - 2z \cos \left(\frac{2r - 1}{2n} \pi\right) + 1\right) \left(z^2 + 2z \cos \left(\frac{2r - 1}{2n} \pi\right) + 1\right).
          \end{align*}

          Let \(z = i\), we have
          \begin{align*}
              \LHS & = \sum_{r = 0}^{n - 1} (-1)^r i^{2r}  \\
                   & = \sum_{r = 0}^{n - 1} (-1)^r (i^2)^r \\
                   & = \sum_{r = 0}^{n - 1} (-1)^r (-1)^r  \\
                   & = \sum_{r = 0}^{n - 1} [(-1)(-1)]^r   \\
                   & = \sum_{r = 0}^{n - 1} 1              \\
                   & = n,
          \end{align*}
          and
          \begin{align*}
              \RHS & = \prod_{r = 1}^{\frac{n - 1}{2}} \left(i^2 - 2i \cos \left(\frac{2r - 1}{2n} \pi\right) + 1\right) \left(i^2 + 2i \cos \left(\frac{2r - 1}{2n} \pi\right) + 1\right) \\
                   & = \prod_{r = 1}^{\frac{n - 1}{2}} (-2i \cos \left(\frac{2r - 1}{2n} \pi\right)) (2i \cos \left(\frac{2r - 1}{2n} \pi\right))                                          \\
                   & = \prod_{r = 1}^{\frac{n - 1}{2}} 4 \cos^2 \left(\frac{2r - 1}{2n} \pi\right)                                                                                         \\
                   & = 2^{n - 1} \prod_{r = 1}^{\frac{n - 1}{2}} \cos^2 \left(\frac{2r - 1}{2n} \pi\right).
          \end{align*}

          This gives
          \[
              \prod_{r = 1}^{\frac{n - 1}{2}} \cos^2 \left(\frac{2r - 1}{2n} \pi\right) = n 2^{1 - n},
          \]
          exactly as desired.
\end{enumerate}