\Question{\currfilebase}

\begin{center}
    \input{\currfiledir 6-diag.tex}
\end{center}

In the diagram, due to the triangular inequality, we must have \(AB \leq OA + OB\), and hence \(\abs*{z - w} \leq \abs*{z} + \abs*{w}\) as desired.

\begin{enumerate}
    \item We have
          \begin{align*}
              \LHS & = \abs*{z - w}^2                                    \\
                   & = (z - w)(z - w)^*                                  \\
                   & = (z - w)(z^* - w^*)                                \\
                   & = z z^* + w w^* - z w^* - z^* w                     \\
                   & = \abs*{z}^2 + \abs*{w}^2 - (E - 2\abs*{zw})        \\
                   & = \abs*{z}^2 + 2 \abs*{z} \abs*{w} + \abs*{w}^2 - E \\
                   & = (\abs*{z} + \abs*{w})^2 - E                       \\
                   & = \RHS,
          \end{align*}
          exactly as desired.

          Since \(\abs*{z - w}\), \(\abs*{z}\) and \(\abs*{w}\) are all real, so must be \(\abs*{z - w}^2\) and \((\abs*{z} + \abs*{w})^2\), and so \(E\) must be real.

          Furthermore, we have
          \[
              E = (\abs*{z} + \abs*{w})^2 - \abs*{z - w}^2,
          \]
          and by the inequality \(\abs*{z} + \abs*{w} \geq \abs*{z - w} \geq 0\), we can conclude
          \[
              (\abs*{z} + \abs*{w})^2 \geq \abs*{z - w}^2,
          \]
          and hence \(E\) must be non-negative.

    \item We have
          \begin{align*}
              \LHS & = \abs*{1 - z w^*}^2                  \\
                   & = (1 - z w^*)(1 - z w^*)^*            \\
                   & = (1 - z w^*)(1 - z^* w)              \\
                   & = 1 - z^* w - z w^* + z w z^* w^*     \\
                   & = 1 - (E - 2 \abs*{zw}) + zw (zw)^*   \\
                   & = 1 - (E - 2 \abs*{zw}) + \abs*{zw}^2 \\
                   & = 1 + 2 \abs*{zw} + \abs*{zw}^2 - E   \\
                   & = (1 + \abs*{zw})^2 - E               \\
                   & = \RHS.
          \end{align*}
\end{enumerate}

If we square both sides of the desired inequality (since both sides are non-negative this is reversible), we have
\[
    \frac{\abs*{z - w}^2}{\abs*{1 - zw^*}^2} \leq \frac{\left(\abs*{z} + \abs*{w}\right)^2}{\left(1 + \abs*{zw}\right)^2},
\]
which is equivalent to showing
\[
    \frac{\left(\abs*{z} + \abs*{w}\right)^2 - E}{\left(1 + \abs*{zw}\right)^2 - E} \leq \frac{\left(\abs*{z} + \abs*{w}\right)^2}{\left(1 + \abs*{zw}\right)^2}.
\]

We introduce a lemma. If \(a > c \geq 0\) and \(a > b\), then
\[
    \frac{b - c}{a - c} \leq \frac{b}{a}.
\]

The proof of this is as follows. We cross-multiply the inequality to give (since \(a \geq a - c > 0\) this is reversible)
\[
    a(b - c) \leq  b (a - c),
\]
which is equivalent to
\[
    ac \geq bc,
\]
and this must be true given \(c \geq 0\) and \(a > b\).

Now, since \(\abs*{z} > 1\), \(\abs*{w} > 1\), we have
\[
    (\abs*{z} - 1)(\abs*{w} - 1) = 1 + \abs*{zw} - \abs*{z} - \abs*{w} > 0,
\]
which means
\[
    1 + \abs*{zw} > \abs*{z} + \abs*{w},
\]
and since both are non-negative we have
\[
    (1 + \abs*{zw})^2 > (\abs*{z} + \abs*{w})^2.
\]

Now, using this lemma, let \(a = (1 + \abs*{zw})^2, b = (\abs*{z} + \abs*{w})^2, c = E\). \(a > b\) is as shown in above, and \(c \geq 0\) is shown in part 1. \(a > c\) since \(a - c = \abs*{1 - zw^*}^2 \geq 0\), and the equal sign holds if and only if \(\abs*{zw^*} = \abs*{zw} = 1\), which must not hold if \(\abs*{z} > 1\) and \(\abs*{w} > 1\) since this gives \(\abs*{zw} = \abs*{z} \abs*{w} > 1\).

Therefore, we must have
\[
    \frac{\left(\abs*{z} + \abs*{w}\right)^2 - E}{\left(1 + \abs*{zw}\right)^2 - E} \leq \frac{\left(\abs*{z} + \abs*{w}\right)^2}{\left(1 + \abs*{zw}\right)^2},
\]
which gives exactly what is desired.

This also holds for \(\abs*{z} < 1\) and \(\abs*{w} < 1\) since from this \((\abs*{z} - 1)(\abs*{w} - 1) > 0\) still holds, so \((1 + \abs*{zw})^2 > (\abs*{z} + \abs*{w})^2\) remains true, and \(\abs*{zw} = \abs*{z}\abs*{w} < 1\) so \(\abs*{zw} \neq 1\) remains true. The exact argument is still valid.