\Question{\currfilebase}

\begin{enumerate}
    \item We notice that
          \begin{align*}
              \DiffFrac{E}{x} & = 2 \cdot \DiffFrac{y}{x} \cdot \NdiffFrac{2}{y}{x} + 2 y^3 \DiffFrac{y}{x} \\
                              & = 2 \cdot \DiffFrac{y}{x} \cdot \left(\NdiffFrac{2}{y}{x} + y^3\right)      \\
                              & = 0,
          \end{align*}
          and so \(E\) must be constant.

          So hence
          \begin{align*}
              E(x) & = E(0)              \\
                   & = 0^2 + \frac{1}{2} \\
                   & = \frac{1}{2}.
          \end{align*}

          Therefore,
          \[
              y^4 = 2\left[E(x) - \left(\DiffFrac{y}{x}\right)^2\right] \leq 2 E(x) = 1,
          \]
          and hence
          \[
              \abs*{y(x)} \leq 1.
          \]

    \item We notice that
          \begin{align*}
              \DiffFrac{E}{x} & = 2 \cdot \DiffFrac{v}{x} \cdot \NdiffFrac{2}{v}{x} + 2 \sinh v \DiffFrac{v}{x} \\
                              & = 2 \DiffFrac{v}{x} \cdot \left(\NdiffFrac{2}{v}{x} + \sinh v\right)            \\
                              & = 2 \DiffFrac{v}{x} \cdot \left(-x \DiffFrac{v}{x}\right)                       \\
                              & = -2x \left(\DiffFrac{v}{x}\right)^2,
          \end{align*}
          so when \(x \geq 0\), since \(\left(\DiffFrac{v}{x}\right)^2 \geq 0\), we must have
          \[
              \DiffFrac{E}{x} \leq 0.
          \]

          Therefore, for \(x \geq 0\), \(E(x) \leq E(0) = 0^2 + 2 \cosh \ln 3 = 3 + \frac{1}{3} = \frac{10}{3}\). Hence,
          \begin{align*}
              \cosh v(x) & = \frac{E(x) - \left(\DiffFrac{v}{x}\right)^2}{2} \\
                         & \leq \frac{\frac{10}{3}}{2}                       \\
                         & = \frac{5}{3}.
          \end{align*}

    \item Notice that
          \begin{align*}
              \DiffOp{x} \left(\DiffFrac{w}{x}\right)^2 & = 2 \cdot \DiffFrac{v}{x} \cdot \NdiffFrac{2}{v}{x}                                                                                               \\
                                                        & = - 2 \cdot \DiffFrac{w}{x} \cdot \left[\left(5 \cosh x - 4 \sinh x - 3\right) \cdot \DiffFrac{w}{x} + \left(w \cosh w + 2 \sinh w\right)\right].
          \end{align*}

          We also notice that
          \begin{align*}
              \int (w \cosh w + 2 \sinh w) \Diff w & = \int w \cosh w \Diff w + 2 \cosh w               \\
                                                   & = \int w \Diff \sinh w + 2 \cosh w + C             \\
                                                   & = w \sinh w - \int \sinh w \Diff w + 2 \cosh w + C \\
                                                   & = w \sinh w - \cosh w + 2 \cosh w + C              \\
                                                   & = w \sinh w + \cosh w + C,
          \end{align*}
          so consider the function
          \[
              E(x) = \left(\DiffFrac{w}{x}\right)^2 + 2(w \sinh w + \cosh w),
          \]
          and we have
          \begin{align*}
              \DiffFrac{E}{x} & = - 2 \cdot \DiffFrac{w}{x} \cdot \left[\left(5 \cosh x - 4 \sinh x - 3\right) \cdot \DiffFrac{w}{x} + \left(w \cosh w + 2 \sinh w\right) - \left(w \cosh w + 2 \sinh w\right)\right] \\
                              & = -2 \left(\DiffFrac{w}{x}\right)^2 \left(5 \cosh x - 4 \sinh x - 3\right)                                                                                                            \\
                              & = - \left(\DiffFrac{w}{x}\right)^2 \left[5 \left(e^x + e^{-x}\right) - 4 \left(e^x - e^{-x}\right) - 6\right]                                                                         \\
                              & = - \left(\DiffFrac{w}{x}\right)^2 \left(e^x + 9e^{-x} - 6\right)                                                                                                                     \\
                              & = - e^{-x} \left(\DiffFrac{w}{x}\right)^2 (e^x - 3)^2                                                                                                                                 \\
                              & \leq 0.
          \end{align*}

          Hence,
          \[
              E(x) \leq E(0) = \left(\frac{1}{\sqrt{2}}\right)^2 + 2 (0 \sinh 0 + \cosh 0) = \frac{1}{2} + 2 = \frac{5}{2},
          \]
          for \(x \geq 0\).

          Therefore,
          \[
              \frac{5}{2} \geq \left(\DiffFrac{w}{x}\right)^2 + 2(w \sinh w + \cosh w),
          \]
          and hence
          \[
              2(w \sinh w + \cosh w) \leq \frac{5}{2}
          \]
          for \(x \geq 0\) since squares are always non-negative.

          Hence,
          \[
              \cosh w \leq \frac{5}{4} - w \sinh w \leq \frac{5}{4}
          \]
          for \(x \geq 0\), the second inequality being true since \(w \sinh w \geq 0\) since \(\sinh w\) and \(w\) always take the same sign, as desired.
\end{enumerate}