\Question{\currfilebase}

We have
\begin{align*}
    \DiffFrac{z}{x} & = n \cdot y^{n - 1} \cdot \DiffFrac{y}{x} \cdot \left(\DiffFrac{y}{x}\right)^2 + y^n \cdot 2 \cdot \DiffFrac{y}{x} \cdot \NdiffFrac{2}{y}{x} \\
                    & = y^{n - 1} \DiffFrac{y}{x} \left[n \left(\DiffFrac{y}{x}\right)^2 + 2y \NdiffFrac{2}{y}{x}\right],
\end{align*}
as desired.

\begin{enumerate}
    \item Let \(n = 1\), we have \(z = y \left(\DiffFrac{y}{x}\right)^2\), and
          \[
              \DiffFrac{z}{x} = \DiffFrac{y}{x} \left[\left(\DiffFrac{y}{x}\right)^2 + 2y \NdiffFrac{2}{y}{x}\right].
          \]

          Hence, the differential equation
          \[
              \left(\DiffFrac{y}{x}\right)^2 + 2y \NdiffFrac{2}{y}{x} = \sqrt{y}
          \]
          simplifies to
          \[
              \frac{\DiffFrac{z}{x}}{\DiffFrac{y}{x}} = \sqrt{y},
          \]
          and hence
          \[
              \DiffFrac{z}{y} = \sqrt{y}.
          \]

          Hence, by integration,
          \[
              z = \frac{2}{3} y^{\frac{3}{2}} + C.
          \]

          When \(x = 0\), \(y = 1\) and \(\DiffFrac{y}{x} = 0\), and hence \(z = 0\). Hence,
          \[
              0 = \frac{2}{3} + C,
          \]
          and therefore \(C = -\frac{2}{3}\).

          We therefore have
          \[
              y \left(\DiffFrac{y}{x}\right)^2 =\frac{2}{3} y^{\frac{3}{2}} - \frac{2}{3},
          \]
          and hence
          \[
              \DiffFrac{y}{x} = \sqrt{\frac{2}{3} \left(\sqrt{y} - \frac{1}{y}\right)}.
          \]

          Rearrangement gives
          \[
              \frac{\sqrt{y} \Diff y}{\sqrt{y^{\frac{3}{2}} - 1}} = \sqrt{\frac{2}{3}} \Diff x.
          \]

          Notice that
          \begin{align*}
              \DiffFrac{\sqrt{y^{\frac{3}{2}} - 1}}{y} & = \frac{1}{2} \cdot \frac{1}{\sqrt{y^{\frac{3}{2}} - 1}} \cdot \frac{3}{2} \cdot \sqrt{y} \\
                                                       & = \frac{3}{4} \cdot \frac{\sqrt{y}}{\sqrt{y^{\frac{3}{2}} - 1}},
          \end{align*}
          and hence by integration
          \[
              \frac{4}{3} \cdot \sqrt{y^{\frac{3}{2}} - 1} = \sqrt{\frac{2}{3}} x + C.
          \]

          When \(x = 0, y = 1\), and hence \(C = 0\). Therefore,
          \[
              \sqrt{y^{\frac{3}{2}} - 1} = \sqrt{\frac{3}{8}} x,
          \]
          and hence
          \[
              y^{\frac{3}{2}} = \frac{3}{8} x^2 + 1,
          \]
          and hence
          \[
              y = \left(\frac{3}{8}x^2 + 1\right)^{\frac{2}{3}},
          \]
          as desired.

    \item Let \(n = -2\), we have \(z = y^{-2} \left(\DiffFrac{y}{x}\right)^2\), and
          \[
              \DiffFrac{z}{x} = -2y^{-3} \DiffFrac{y}{x} \left[\left(\DiffFrac{y}{x}\right)^2 - y \NdiffFrac{2}{y}{x}\right].
          \]

          Hence, the differential equation
          \[
              \left(\DiffFrac{y}{x}\right)^2 - y \NdiffFrac{2}{y}{x} + y^2 = 0
          \]
          simplifies to
          \[
              \frac{\DiffFrac{z}{x}}{-2y^{-3} \DiffFrac{y}{x}} + y^2 = 0,
          \]
          which gives
          \[
              \DiffFrac{z}{y}  = \frac{2}{y}.
          \]

          By integration on both sides, we have
          \[
              z = 2 \ln y + C,
          \]
          and when \(x = 0\), \(y = 1\), \(\DiffFrac{y}{x} = 0\), which gives \(z = 0\). Hence, \(C = 0\), and
          \[
              y^{-2} \left(\DiffFrac{y}{x}\right)^2 = 2 \ln y,
          \]
          which gives
          \[
              \DiffFrac{y}{x} = y\sqrt{2 \ln y},
          \]
          and therefore,
          \[
              \frac{\Diff y}{y \sqrt{\ln y}} = \sqrt{2} \Diff x.
          \]

          By integration,
          \[
              \int \frac{\Diff y}{y \sqrt{\ln y}} = \int \frac{\Diff \ln y}{\sqrt{\ln y}} = 2 \sqrt{\ln y} + C,
          \]
          and hence
          \[
              2 \sqrt{\ln y} = \sqrt{2} x + C.
          \]

          When \(x = 0\), \(y = 1\), so \(C = 0\), and hence
          \[
              \sqrt{\ln y} = \frac{x}{\sqrt{2}},
          \]
          and therefore, the solution to the original differential equation is
          \[
              y = e^{\frac{x^2}{2}}.
          \]
\end{enumerate}