\Question{\currfilebase}

\begin{enumerate}
    \item By the formula for difference of two squares, we have
          \begin{align*}
              (1 - x)(1 + x)(1 + x^2)(1 + x^4) \cdots (1 + x^{2^n}) & = (1 - x^2)(1 + x^2)(1 + x^4) \cdots (1 + x^{2^n}) \\
                                                                    & = (1 - x^4)(1 + x^4) \cdots (1 + x^{2^n})          \\
                                                                    & = \cdots                                           \\
                                                                    & = 1 - x^{2^{n + 1}}.
          \end{align*}

          This means,
          \[
              1 = (1 - x)(1 + x)(1 + x^2)(1 + x^4) \cdots (1 + x^{2^n}) + x^{2^{n + 1}},
          \]
          and dividing both sides by \(1 - x\) gives
          \[
              \frac{1}{1 - x} = (1 + x)(1 + x^2)(1 + x^4) \cdots (1 + x^{2^n}) + \frac{x^{2^{n + 1}}}{1 - x}.
          \]

          Rearranging and taking natural logs on both sides, we have
          \[
              \ln(1 - x^{2^{n + 1}}) - \ln(1 - x) = \sum_{k = 0}^{n} \ln(1 + x^{2^{k}}),
          \]
          and therefore,
          \[
              \ln(1 - x) = -\sum_{k = 0}^{n} \ln(1 + x^{2^{k}}) + \ln(1 - x^{2^{n + 1}}).
          \]

          Let \(n \to \infty\). \(2^{n + 1} \to \infty\), and since \(\abs*{x} < 1\), we have \(x^{2^{n + 1}} \to 0\), and hence
          \[
              \ln(1 - x) = -\sum_{k = 0}^{\infty} \ln(1 + x^{2^{k}}) + \ln(1) = -\sum_{k = 0}^{\infty} \ln(1 + x^{2^{k}}),
          \]
          as desired.

          Differentiating both sides with respect to \(x\), we have
          \[
              - \frac{1}{1 - x} = - \sum_{k = 0}^{\infty} \frac{2^k x^{2^k - 1}}{1 + x^{2^k}},
          \]
          and hence
          \[
              \frac{1}{1 - x} = \sum_{k = 0}^{\infty} \frac{2^k x^{2^k - 1}}{1 + x^{2^k}},
          \]
          exactly as desired.

    \item Notice that
          \begin{align*}
               & \phantom{=} (1 + x + x^2) (1 - x + x^2) (1 - x^2 + x^4) (1 - x^4 + x^8) \cdots (1 - x^{2^{n - 1}} + x^{2^n}) \\
               & = ((1 + x^2)^2 - x^2) (1 - x^2 + x^4) (1 - x^4 + x^8) \cdots (1 - x^{2^{n - 1}} + x^{2^n})                   \\
               & = (1 + x^2 + x^4) (1 - x^2 + x^4) (1 - x^4 + x^8) \cdots (1 - x^{2^{n - 1}} + x^{2^n})                       \\
               & = ((1 + x^4)^2 - (x^2)^2) (1 - x^4 + x^8) \cdots (1 - x^{2^{n - 1}} + x^{2^n})                               \\
               & = (1 + x^4 + x^8)(1 - x^4 + x^8) \cdots (1 - x^{2^{n - 1}} + x^{2^n})                                        \\
               & = \cdots                                                                                                     \\
               & = 1 + x^{2^n} + x^{2^{n + 1}}.
          \end{align*}

          Therefore,
          \[
              1 = (1 + x + x^2) (1 - x + x^2) (1 - x^2 + x^4) (1 - x^4 + x^8) \cdots (1 - x^{2^{n - 1}} + x^{2^n}) - x^{2^n} - x^{2^{n + 1}},
          \]
          and hence
          \[
              \frac{1}{1 + x + x^2} = (1 - x + x^2) (1 - x^2 + x^4) (1 - x^4 + x^8) \cdots (1 - x^{2^{n - 1}} + x^{2^n}) - \frac{x^{2^n} + x^{2^{n + 1}}}{1 + x + x^2}.
          \]

          Rearranging and taking natural logs on both sides, we have
          \[
              \ln(1 + x^{2^n} + x^{2^{n + 1}}) - \ln (1 + x + x^2) = \sum_{k = 1}^{n} \ln(1 - x^{2^{k - 1}} + x^{2^k}),
          \]
          and hence
          \[
              \ln (1 + x + x^2) = -\sum_{k = 1}^{n} \ln(1 - x^{2^{k - 1}} + x^{2^k}) + \ln(1 + x^{2^n} + x^{2^{n + 1}}).
          \]

          Let \(n \to \infty\), we have \(2^n, 2^{n + 1} \to \infty\), and since \(\abs*{x} < 1\), we must have \(x^{2^n}, x^{2^{n + 1}} \to \infty\), and hence \(\ln(1 + x^{2^n} + x^{2^{n + 1}}) \to 0\). Hence,
          \[
              \ln (1 + x + x^2) = - \sum_{k = 1}^{\infty} \ln(1 - x^{2^{k - 1}} + x^{2^k}).
          \]

          Differentiating both sides with respect to \(x\), we get
          \[
              \frac{1 + 2x}{1 + x + x^2} = - \sum_{k = 1}^{\infty} \frac{- 2^{k - 1} x^{2^{k - 1} - 1} + 2^{k} x^{2^{k} - 1} }{1 - x^{2^{k - 1}} + x^{2^k}} = \sum_{k = 1}^{\infty} \frac{2^{k - 1} x^{2^{k - 1} - 1} - 2^{k} x^{2^{k} - 1} }{1 - x^{2^{k - 1}} + x^{2^k}},
          \]
          which is exactly what is desired.
\end{enumerate}