\Question{\currfilebase}

\begin{enumerate}
    \item Let \(u = \sqrt{x}\), we have \(x = u^2\), and hence \(\Diff x = 2u \Diff u\).

          When \(x = 0, u = 0\), and when \(x = 1, u = 1\).

          Therefore,
          \begin{align*}
              \int_{0}^{1} f\left(\sqrt{x}\right)\Diff x & = \int_{0}^{1} f(u) \cdot 2u \Diff u \\
                                                         & = 2 \int_{0}^{1} u f(u) \Diff u      \\
                                                         & = 2 \int_{0}^{1} x f(x) \Diff x.
          \end{align*}

    \item We have
          \begin{align*}
              \int_{0}^{1} \left(g(x)\right)^2 \Diff x & = \int_{0}^{1} g\left(\sqrt{x}\right) \Diff x - \frac{1}{3} \\
                                                       & = 2 \int_{0}^{1} x g(x) \Diff x - \int_{0}^{1} x^2 \Diff x,
          \end{align*}
          and hence
          \begin{align*}
              \int_{0}^{1} \left[\left(g(x)\right)^2 - 2x g(x) + x^2\right] \Diff x & = 0  \\
              \int_{0}^{1} \left(g(x) - x\right)^2 \Diff x                          & = 0.
          \end{align*}

          We have \(\left(g(x) - x\right)^2 \geq 0\) for all \(0 \leq x \leq 1\), and since \(g\) is continuous, we must have \(g(x) - x = 0\) for all \(0 \leq x \leq 1\) for the integral to evaluate to \(0\).

          Hence, \(g(x) = x\) for \(0 \leq x \leq 1\).

    \item Using integration by parts, we have
          \begin{align*}
              \int_{0}^{1} h(x) \Diff x & = \left[x h(x)\right]_{0}^{1} - \int_{0}^{1} x \Diff h(x)    \\
                                        & = 1 \cdot h(1) - 0 \cdot h(0) - \int_{0}^{1} x h'(x) \Diff x \\
                                        & = h(1) - \int_{0}^{1} x h'(x) \Diff x.
          \end{align*}

          Hence,
          \begin{align*}
              \int_{0}^{1} \left(h'(x)\right)^2 \Diff x & = 2h(1) - 2 \int_{0}^{1} h(x) \Diff x - \frac{1}{3}                         \\
                                                        & = 2 h(1) - 2 \left[h(1) - \int_{0}^{1} x h'(x) \Diff x\right] - \frac{1}{3} \\
                                                        & = 2 \int_{0}^{1} x h'(x) \Diff x - \frac{1}{3}                              \\
                                                        & = 2 \int_{0}^{1} x h'(x) \Diff x - \int_{0}^{1} x^2 \Diff x.
          \end{align*}

          Therefore, similar to the previous part, we have \(h'(x) = x\) for \(0 \leq x \leq 1\), and hence \(h(x) = \frac{x^2}{2} + h(0) = \frac{x^2}{2}\) for \(0 \leq x \leq 1\).

    \item First, we notice that
          \begin{align*}
              \int_{0}^{1} e^{-ax} \Diff x & = - \frac{1}{a} \left[e^{-ax}\right]_{0}^{1}  \\
                                           & = - \frac{1}{a} \cdot \left[e^{-a} - 1\right] \\
                                           & = - \frac{e^{-a}}{a} + \frac{1}{a}.
          \end{align*}

          Hence,
          \begin{align*}
              \int_{0}^{1} e^{ax} \left(k(x)\right)^2 \Diff x                                           & = 2 \int_{0}^{1} k(x) \Diff x - \int_{0}^{1} e^{-ax} \Diff x + \frac{1}{a} - \frac{1}{a^2} - \frac{1}{4} \\
              \int_{0}^{1} \left[e^{ax} \left(k(x)\right)^2 - 2 k(x) + e^{-ax}\right] \Diff x           & = - \frac{1}{a^2} + \frac{1}{a} - \frac{1}{4}                                                            \\
              \int_{0}^{1} e^{-ax} \left[e^{2ax} \left(k(x)\right)^2 - 2 e^{ax} k(x) + 1\right] \Diff x & = - \left(\frac{1}{a} - \frac{1}{2}\right)^2                                                             \\
              \int_{0}^{1} e^{-ax} \left(e^{ax} k(x)- 1\right)^2 \Diff x                                & = - \left(\frac{1}{a} - \frac{1}{2}\right)^2.
          \end{align*}

          Since \(e^{-ax} > 0\), and \(\left(e^{ax} k(x) - 1\right)^2 \geq 0\), the integrand must be non-negative, and hence
          \[
              \int_{0}^{1} e^{-ax} \left(e^{ax} k(x)- 1\right)^2 \Diff x \geq 0,
          \]
          meaning
          \[
              \left(\frac{1}{a} - \frac{1}{2}\right)^2 \leq 0.
          \]

          However, since this is a square, it is non-negative, and it must be the case that \(\left(\frac{1}{a} - \frac{1}{2}\right)^2 = 0\), giving \(\frac{1}{a} = \frac{1}{2}\), and hence \(a = 2\).

          Therefore,
          \[
              \int_{0}^{1} e^{-ax} \left(e^{ax} k(x)- 1\right)^2 \Diff x = 0,
          \]
          and since the integrand is continuous and non-negative over the interval, it must be zero everywhere for \(0 \leq x \leq 1\), and hence
          \[
              e^{ax} k(x) - 1 = 0,
          \]
          giving
          \[
              k(x) = e^{-ax} = e^{-2x}
          \]
          for \(0 \leq x \leq 1\).
\end{enumerate}