\Question{\currfilebase}

\begin{enumerate}
    \item By using the chain rule, we have
          \begin{align*}
              \DiffFrac{y}{x} & = \frac{\Diff y / \Diff t}{\Diff x / \Diff t}               \\
                              & = \frac{12 \cos t - 12 \sin^2 t \cos t}{12 \cos^2 t \sin t} \\
                              & = \frac{\cos t - \sin^2 t \cos t}{\cos^2 t \sin t}          \\
                              & = \frac{1 - \sin^2 t}{\cos t \sin t}                        \\
                              & = \frac{\cos^2 t}{\cos t \sin t}                            \\
                              & = \frac{\cos t}{\sin t}                                     \\
                              & = \cot t.
          \end{align*}

          Hence, at \(t = \phi\), the normal of this curve has gradient \(- \tan \phi\), and hence it has equation
          \begin{align*}
              y - \left(12 \sin \phi - 4 \sin^3 \phi\right)                  & = - \tan \phi \left(x - \left(-4 \cos^3 \phi\right)\right)                   \\
              y - 12 \sin \phi + 4 \sin^3 \phi                               & =  - \tan \phi x - 4 \cos^3 \phi \tan \phi                                   \\
              \cos \phi y - 12 \sin \phi \cos \phi + 4 \sin^3 \phi \cos \phi & = - \sin \phi x - 4 \cos^3 \phi \sin \phi                                    \\
              \sin \phi x + \cos \phi y                                      & = 12 \sin \phi \cos \phi - 4 \sin^3 \phi \cos \phi - 4 \cos^3 \phi \sin \phi \\
              \sin \phi x + \cos \phi y                                      & = 4 \sin \phi \cos \phi \left(3 - \sin^2 \phi - \cos^2 \phi\right)           \\
              \sin \phi x + \cos \phi y                                      & = 8 \sin \phi \cos \phi.
          \end{align*}

          The curve \(x^{\frac{2}{3}} + y^{\frac{2}{3}} = 4\) can be parametrised as \(x = 8 \cos^3 t\) and \(y = 8 \sin^3 t\):
          \begin{align*}
              x^{\frac{2}{3}} + y^{\frac{2}{3}} & = \left(8 \cos^3 t\right)^{\frac{2}{3}} + \left(8 \sin^3 t\right)^{\frac{2}{3}} \\
                                                & = 4 \cos^2 t + 4 \sin^2 t                                                       \\
                                                & = 4.
          \end{align*}

          Hence, the gradient of the tangent at a point is
          \begin{align*}
              \DiffFrac{y}{x} & = \frac{\Diff y / \Diff t}{\Diff x / \Diff t}    \\
                              & = \frac{24 \sin^2 t \cos t}{-24 \cos^2 t \sin t} \\
                              & = - \tan t,
          \end{align*}
          and the equation of the tangent at the point \(t = \phi\) is
          \begin{align*}
              y - 8 \sin^3 \phi                     & = - \tan \phi \left(x - 8 \cos^3 \phi\right)                   \\
              \cos \phi y - 8 \sin^3 \phi \cos \phi & = - \sin \phi x + 8 \cos^3 \phi \sin \phi                      \\
              \sin \phi x + \cos \phi y             & = 8 \sin \phi \cos \phi \left(\sin^2 \phi + \cos^2 \phi\right) \\
              \sin \phi x + \cos \phi y             & = 8 \sin \phi \cos \phi,
          \end{align*}
          which shows the normal to the original curve is the tangent to this new curve at \((8 \cos^3 \phi, 8 \sin^3 \phi)\).

    \item By using the chain rule, we have
          \begin{align*}
              \DiffFrac{y}{x} & = \frac{\Diff y / \Diff t}{\Diff x / \Diff t}                     \\
                              & = \frac{\cos t - \cos t + t \sin t}{- \sin t + \sin t + t \cos t} \\
                              & = \frac{t \sin t}{t \cos t}                                       \\
                              & = \tan t.
          \end{align*}

          Hence, at \(t = \phi\), the normal of this curve has gradient \(- \cot \phi\), and hence it has equation
          \begin{align*}
              y - \left(\sin \phi - \phi \cos \phi\right)          & = - \cot \phi \left(x - \left(\cos \phi + \phi \sin \phi\right)\right) \\
              \sin \phi y - \sin^2 \phi + \phi \sin \phi \cos \phi & = - \cos \phi x + \cos^2 \phi + \phi \sin \phi \cos \phi               \\
              \cos \phi x + \sin \phi y                            & = \sin^2 \phi + \cos^2 \phi                                            \\
              \cos \phi x + \sin \phi y                            & = 1.
          \end{align*}

          The distance of this normal to the origin is
          \[
              \frac{\abs*{\cos \phi \cdot 0 + \sin \phi \cdot 0 - 1}}{\sqrt{\cos^2 \phi + \sin^2 \phi}} = 1,
          \]
          which is a constant, and hence this curve is tangent to the unit circle \(x^2 + y^2 = 1\).
\end{enumerate}